\documentclass[a4paper]{article}
\usepackage{amsmath}

\begin{document}

\section{Generalised Transition Rate Equation}

\begin{equation}
T^{j\rightarrow i} = \left(u_i r_{i-1} \frac{n_{i-1}}{N} + \left(1 - u_{i+1} \right) r_i \frac{n_i}{N} \right) \frac{n_j}{\bar{r}}
\end{equation}

When setting up the system, $u_0 = 0$ and $u_{N+1} = 0$ must be defined in order to stop cells mutating past the maximum number of mutations. 

\subsection{Diffusion with Drift Derivation}

Taking the large $N$ limit. 

\begin{align*}
 \dot{x} _i & = \frac{1}{N} \left[ \sum _j T^{j \rightarrow i} - T^{i \rightarrow j} \right]\\
\end{align*}

Using the generalised transition rate equation:

\begin{align*}
\bar{r} \dot{x}_i & = \sum _j u _i r_{i-1} x_{i-1} x_j - u_j r_{j-1} x_{j-1} x_{i} + x_j x_i \left[ ( 1- u_{i+1} ) r_i - (1 - u_{j+1} ) r_j \right] \\
\alpha & = u _i r _{i-1} \\
\beta & = u_j r_{j-1} \\
\gamma & = ( 1 - u_{i+1} ) r_i - ( 1- u_{j+1} )r_j ) \\
\bar{r} \dot{x}_i & = \sum _j \alpha x_j x_{i-1} - \beta x_{j-1} x_i + \gamma x_j x_i \\
\end{align*}

In a flat fitness and mutation landscape, away from the absorbing state $ u_i, r_i = 1 \forall i$. 
From this $\alpha = 1, \beta = 1, \gamma = 0, \bar{r} = 1$.

\begin{align*}
\dot{\rho} _i & = \sum _j \rho _j \rho _{i-1} - \rho _{j-1} \rho _{i} \\
\end{align*}

We now want to expand this sum in order to simplify; 

\begin{align*}
\dot{\rho} _i & = \rho _0 \rho _{i - 1} + ( \rho _1 \rho _{i-1} - \rho _0 \rho _i ) + ( \rho _2 \rho _{i-1} - \rho _1 \rho _i ) + ... + ( \rho _{N - 1} \rho _{i-1} - \rho _{N-2} \rho _i ) + ( \rho _N \rho _{i-1} - \rho _{N-1} \rho _i ) \\
& = \rho _0 ( \rho _{i-1} - \rho _i ) + \rho _1 ( \rho _{i-1} - \rho _i ) + ... + \rho _N \rho _{i-1} \\
& = \sum _k ^{N -1} ( \rho _{i-1} - \rho _i ) \rho _k + \rho _N \rho _{i-1} \\
& = ( \rho _{i-1} - \rho _i ) ( 1 - \rho _N ) + \rho _N \rho _{i-1} \\
& = \rho _{i-1} + ( \rho _N - 1) \rho _i \\
\dot{\rho} _i & = \rho _{i-1} + (\rho _N - 1 ) \rho _i
\end{align*} 

In the large mutation limit $\rho _N \rightarrow 0 $.

\begin{equation}
\dot{\rho} _i  = \rho _{i-1} - \rho _i 
\end{equation} 

We might be breaking our previous assumptions, but for $i=0$:

\begin{align*}
\dot{\rho} _0 & = 0 - \rho _0 \\
\rho _0 & = A e^{-t} \\
A & = 1 \\
\rho _0 & = e^{-t} \\
\end{align*}

This gives us the first step in solving generally. 

\begin{align*}
\dot{\rho} _1 & = \rho _0 - \rho _1 \\
& = e^{-t} - \rho _1 \\
\rho _1 & = t e ^{-t} \\
\dot{\rho} _2 & = \rho _1 - \rho _2 \\
\rho _2 & = \frac{1}{2} e^{-t} t ^2 \\
\end{align*}

From this we can see that the general solution for $\rho _i$; 

\begin{equation}
\rho _i = \frac{t ^i}{i!} e ^{-t} 
\end{equation}




\end{document}