\documentclass[a4paper]{article}
\usepackage{amsmath}

\begin{document}

\section{Generalised Transition Rate Equation}

\begin{equation}
T^{j\rightarrow i} = \left(u_i r_{i-1} \frac{n_{i-1}}{N} + \left(1 - u_{i+1} \right) r_i \frac{n_i}{N} \right) \frac{n_j}{\bar{r}}
\end{equation}

When setting up the system, $u_0 = 0$ and $u_{N+1} = 0$ must be defined in order to stop cells mutating past the maximum number of mutations. 

$\frac{n_j}{\bar{r}}$ is selected to die.
$u_i r_{i-1} \frac{n_{i-1}}{N}$ is selected to mutate and gain a mutation. I.e. a cell with one less mutation is birthed with a mutation. 
$\left(1 - u_{i+1} \right) r_i \frac{n_i}{N}$ A $n_i$ cell is born and doesn't obtain a mutation.

\subsection{Diffusion with Drift Derivation}

Taking the large $N$ limit. 

\begin{align*}
 \dot{x} _i & = \frac{1}{N} \left[ \sum _j T^{j \rightarrow i} - T^{i \rightarrow j} \right]\\
\end{align*}

Using the generalised transition rate equation:

\begin{align*}
\bar{r} \dot{x}_i & = \sum _j u _i r_{i-1} x_{i-1} x_j - u_j r_{j-1} x_{j-1} x_{i} + x_j x_i \left[ ( 1- u_{i+1} ) r_i - (1 - u_{j+1} ) r_j \right] \\
\alpha & = u _i r _{i-1} \\
\beta & = u_j r_{j-1} \\
\gamma & = ( 1 - u_{i+1} ) r_i - ( 1- u_{j+1} )r_j ) \\
\bar{r} \dot{x}_i & = \sum _j \alpha x_j x_{i-1} - \beta x_{j-1} x_i + \gamma x_j x_i \\
\end{align*}

In a flat fitness and mutation landscape, away from the absorbing state $ u_i, r_i = 1 \forall i$. 
From this $\alpha = 1, \beta = 1, \gamma = 0, \bar{r} = 1$.

\begin{align*}
\dot{\rho} _i & = \sum _j \rho _j \rho _{i-1} - \rho _{j-1} \rho _{i} \\
\end{align*}

We now want to expand this sum in order to simplify; 

\begin{align*}
\dot{\rho} _i & = \rho _0 \rho _{i - 1} + ( \rho _1 \rho _{i-1} - \rho _0 \rho _i ) + ( \rho _2 \rho _{i-1} - \rho _1 \rho _i ) + ... + ( \rho _{N - 1} \rho _{i-1} - \rho _{N-2} \rho _i ) + ( \rho _N \rho _{i-1} - \rho _{N-1} \rho _i ) \\
& = \rho _0 ( \rho _{i-1} - \rho _i ) + \rho _1 ( \rho _{i-1} - \rho _i ) + ... + \rho _N \rho _{i-1} \\
& = \sum _k ^{N -1} ( \rho _{i-1} - \rho _i ) \rho _k + \rho _N \rho _{i-1} \\
& = ( \rho _{i-1} - \rho _i ) ( 1 - \rho _N ) + \rho _N \rho _{i-1} \\
& = \rho _{i-1} + ( \rho _N - 1) \rho _i \\
\dot{\rho} _i & = \rho _{i-1} + (\rho _N - 1 ) \rho _i
\end{align*} 

In the large mutation limit $\rho _N \rightarrow 0 $.

\begin{equation}
\dot{\rho} _i  = \rho _{i-1} - \rho _i 
\end{equation} 

We might be breaking our previous assumptions, but for $i=0$:

\begin{align*}
\dot{\rho} _0 & = 0 - \rho _0 \\
\rho _0 & = A e^{-t} \\
A & = 1 \\
\rho _0 & = e^{-t} \\
\end{align*}

This gives us the first step in solving generally. 

\begin{align*}
\dot{\rho} _1 & = \rho _0 - \rho _1 \\
& = e^{-t} - \rho _1 \\
\rho _1 & = t e ^{-t} \\
\dot{\rho} _2 & = \rho _1 - \rho _2 \\
\rho _2 & = \frac{1}{2} e^{-t} t ^2 \\
\end{align*}

From this we can see that the general solution for $\rho _i$; 

\begin{equation}
\rho _i = \frac{t ^i}{i!} e ^{-t} 
\end{equation}

\section{Tobias' Model}

Go from state $n$ to $n+1$ with rate $a+b$. 
Go from state $n$ to $n-1$ with rate $a$. 

\begin{align*}
\dot{p_i} & = -a p_i - (a+b ) p_i + (a+b) p_{i-1} + a p_{i+1} \\
& = - (2a + b) p_i +(a+b) p_{i-1} + a p_{i+1} \\
\end{align*}

Lets start with a generating function: 

\begin{align*}
\Phi & = \sum _{n = 0} ^\infty z^n p_n (t) \\
\dot{\Phi} & = \sum _{n=0} ^\infty z^n \dot{p} _n \\
& = \sum _{n = 0} ^\infty z^n \left( (a+b) p_{n-1} - (2a+b) p_n + a p_{n+1} \right) \\
& = - (2a+b) \Phi + a \sum _{n=0} ^\infty z ^n p_{n+1} + (a+b) \sum _{n=0} ^\infty z ^n p_{n-1} \\
& = - (2a + b) \Phi + \frac{a}{z} \Phi + (a+b) z \Phi \\
\end{align*}

Need to get a differential out of this equation though? 

\section{Our Cancer Model Version 2}

\begin{align*}
\dot{x}_i & = \left(u_i r_{i-1} \frac{n_{i-1}}{N} + \left(1 - u_{i+1} \right) r_i \frac{n_i}{N} \right) \frac{n_j}{\bar{r}} - \left(u_j r_{j-1} \frac{n_{j-1}}{N} + \left(1 - u_{j+1} \right) r_j \frac{n_j}{N} \right) \frac{n_i}{\bar{r}} \\
\bar{r} \dot{x}_i & = \left(u_i r_{i-1} x_{i-1} + \left(1 - u_{i+1} \right) r_i x_i \right) x_j - \left(u_j r_{j-1} x_{j-1} + \left(1 - u_{j+1} \right) r_j x_j \right) x_i \\
\\
\bar{r} \dot{x}_0 & = \left( \left(1 - u_{1} \right) r_0 x_0 \right) x_j - \left(u_j r_{j-1} x_{j-1} + \left(1 - u_{j+1} \right) r_j x_j \right) x_0 \\
\\
\end{align*}

\section{Diffusion equation attempt}

\begin{align*}
\bar{r} \dot{x} _i & = \sum _{j \neq i} \left(u_i r_{i-1} x_{i-1} + \left(1 - u_{i+1} \right) r_i x_i \right) x_j - \left(u_j r_{j-1} x_{j-1} + \left(1 - u_{j+1} \right) r_j x_j \right) x_i
\end{align*}

Following this explicitly can reproduce the equations in the Ashcroft paper. 

Now attempt to simplify it: 

\begin{align*}
\bar{r} \dot{x} _i & = \sum _{j \neq i} \left(u_i r_{i-1} x_{i-1} + \left(1 - u_{i+1} \right) r_i x_i \right) x_j - \left(u_j r_{j-1} x_{j-1} + \left(1 - u_{j+1} \right) r_j x_j \right) x_i \\
& = \left(u_i r_{i-1} x_{i-1} + \left(1 - u_{i+1} \right) r_i x_i \right) \sum _{j \neq i} x_j - x_i \sum _{j \neq i} \left(u_j r_{j-1} x_{j-1} + \left(1 - u_{j+1} \right) r_j x_j \right) \\
& = \left(u_i r_{i-1} x_{i-1} + \left(1 - u_{i+1} \right) r_i x_i \right) ( 1- x_i) - x_i \left( \sum _{j \neq i} u _j r_{j-1} x_{j-1} + \sum _{j \neq i} (1 - u_{j+1} ) r_j x_j  \right) \\
& = \left(u_i r_{i-1} x_{i-1} + \left(1 - u_{i+1} \right) r_i x_i \right) ( 1- x_i) - x_i \left( \sum _{j \neq i} u _j r_{j-1} x_{j-1} + \sum _{j \neq i} r_j x_j  - \sum _{j \neq i} r_j x_j u_{j+1}  \right) \\
& = \left(u_i r_{i-1} x_{i-1} + \left(1 - u_{i+1} \right) r_i x_i \right) ( 1- x_i) - x_i \left( \sum _{j \neq i} u _j r_{j-1} x_{j-1} + (\bar{r} - r_i x_i )  - \sum _{j \neq i} r_j x_j u_{j+1}  \right) \\
\end{align*}

\begin{align*}
\bar{u} & = \sum _{i=1} ^{N} u_i r_{i-1} x_{i-1} \\
\mathbf{u} & = (0, u_1, ..., u_{N-1}, 0 ) \\
\sum _{j \neq i} u _j r_{j-1} x_{j-1} - \sum _{j \neq i} u_{j+1}r_j x_j & = ( \bar{u} - u_i r_{i-1} x_{i-1} ) - \sum _{m \neq i +1} u_{m}r_{j-1} x_{j-1} \\
& = ( \bar{u} - u_i r_{i-1} x_{i-1} ) - ( \bar{u} - u_{i+1} r_{i} x_{i}) \\
& = u_{i+1} r_{i} x_{i} - u_i r_{i-1} x_{i-1}
\end{align*}

\begin{align*}
\bar{r} \dot{x} _i & = \left(u_i r_{i-1} x_{i-1} + \left(1 - u_{i+1} \right) r_i x_i \right) ( 1- x_i) - x_i \left( u_{i+1} r_{i} x_{i} - u_i r_{i-1} x_{i-1} + ( \bar{r} - r_i x_i ) \right) \\
& =  \left(u_i r_{i-1} x_{i-1} ( 1- x_i) + \left(1 - u_{i+1} \right) ( 1- x_i)  r_i x_i \right)  -  \left( u_{i+1} r_{i} x ^2_{i} - u_i r_{i-1} x_{i-1} x_i + x_i ( \bar{r} - r_i x_i ) \right) \\
& = \left(u_i r_{i-1} x_{i-1} ( 1- x_i) + \left(1 - u_{i+1} \right) ( 1- x_i)  r_i x_i \right)  -  u_{i+1} r_{i} x ^2_{i} + u_i r_{i-1} x_{i-1} x_i - x_i ( \bar{r} - r_i x_i ) \\
& = \left(u_i r_{i-1} x_{i-1} ( 1- x_i) + \left(1 - u_{i+1} \right) ( 1- x_i)  r_i x_i \right)  -  u_{i+1} r_{i} x ^2_{i} + u_i r_{i-1} x_{i-1} x_i - x_i  \bar{r} + r_i x_i ^2 \\
& = \left(u_i r_{i-1} x_{i-1} - u_i r_{i-1} x_{i-1} x_i + \left(1 - u_{i+1} \right) ( 1- x_i)  r_i x_i \right)  -  u_{i+1} r_{i} x ^2_{i} + u_i r_{i-1} x_{i-1} x_i - x_i  \bar{r} + r_i x_i ^2 \\
& = \left(u_i r_{i-1} x_{i-1} - u_i r_{i-1} x_{i-1} x_i + \left( 1 - u_{i+1} - x_i + u_{i+1} x_i \right)  r_i x_i \right)  -  u_{i+1} r_{i} x ^2_{i} + u_i r_{i-1} x_{i-1} x_i - x_i  \bar{r} + r_i x_i ^2 \\
& = u_i r_{i-1} x_{i-1} - u_i r_{i-1} x_{i-1} x_i +  r_i x_i - r_i x_i u_{i+1} - r_i x^2_i + r_i x ^2_i u_{i+1}  -  u_{i+1} r_{i} x ^2_{i} + u_i r_{i-1} x_{i-1} x_i - x_i  \bar{r} + r_i x_i ^2 \\
& = u_i r_{i-1} x_{i-1} - u_i r_{i-1} x_{i-1} x_i +  r_i x_i - r_i x_i u_{i+1} - r_i x^2_i  + u_i r_{i-1} x_{i-1} x_i - x_i  \bar{r} + r_i x_i ^2 \\
& = u_i r_{i-1} x_{i-1} - u_i r_{i-1} x_{i-1} x_i +  r_i x_i - r_i x_i u_{i+1} + u_i r_{i-1} x_{i-1} x_i - x_i  \bar{r} \\
& = u_i r_{i-1} x_{i-1}  +  r_i x_i - r_i x_i u_{i+1}  - x_i  \bar{r} \\
& = u_i r_{i-1} x_{i-1} + x_i \left( r_i  \left( 1- u_{i+1} \right) - \bar{r} \right) \\ 
\end{align*}

\begin{equation}
\bar{r} \dot{x} _i = u_i r_{i-1} x_{i-1} + x_i \left( r_i  \left( 1- u_{i+1} \right) - \bar{r} \right)
\end{equation}

This reproduces the Ashcroft results as expected. So we can proceed. 

\begin{align}
\bar{r} \dot{x} _0 & = x_0 \left( r_0  \left( 1- u_{1} \right) - \bar{r} \right) \\
\bar{r} \dot{x} _i & = u_i r_{i-1} x_{i-1} + x_i \left( r_i  \left( 1- u_{i+1} \right) - \bar{r} \right) \\
\bar{r} \dot{x} _N & = u_N r_{N-1} x_{N-1} + x_N \left( r_N   - \bar{r} \right)
\end{align}

Assume a constant $r$ and $u$ landscape and just sticking with the middle equation:

\begin{align*}
r \dot{\rho} _i & = u r \rho _{i-1} + \rho _i ( r(1- u) - r) \\
\dot{\rho} _i & = u \rho _{i-1} + \rho _i ( 1-u) - \rho _{i} \\
& = u  ( \rho _{i-1} -  \rho _{i} ) \\
\end{align*}

We then make the change of variables $\rho _i \rightarrow \rho(t, x) $. 

\begin{align*}
\dot{\rho} (t,x ) & = u \left( \rho (t, x - \Delta x) - \rho (t , x) \right) \\
& = u \left( \rho(t,x) - \Delta x \frac{\partial \rho}{\partial x} + \frac{\Delta x ^2}{2} \frac{\partial ^2 \rho}{\partial x ^2}   - \rho (t , x) \right) \\
& = \frac{u \Delta x ^2}{2} \frac{\partial ^2 \rho}{\partial x ^2} - u \Delta x \frac{\partial \rho}{\partial x}
\end{align*}

This resembles the Fokker Plank Equation. 

\section{Solution of Master Equation with Poissonian}

\begin{align*}
\dot{\rho}_0 & = - u \rho _0 \\
\rho _0 & = A e^{-u t} \\
A & = 1 \\
\end{align*}

Then solve for $\rho _1$

\begin{align*}
\dot{\rho} _1 & = u ( \rho _0 - \rho _1 ) \\
& = u \left( e^{-ut} - \rho _1 \right) \\
\dot{\rho}_1 + u \rho _1 & = u e^{-ut} \\
\frac{d}{dt} \left( e ^{ut} \rho \right) & = u \\
\rho _1 & = (ut) e^{-ut} \\
\end{align*}

Doing a proof by induction and we arrive at the standard Poissonian; 

\begin{align*}
\rho _n & = \frac{(ut) ^n}{n!} e^{-ut}
\end{align*}

\section*{Solution with Fourier}

\begin{align*}
\dot{\rho} & = \frac{\tilde{u} \Delta x}{2} \frac{\partial ^2}{\partial x^2} \rho - \tilde{u} \frac{\partial}{\partial x}\rho \\
\tilde{u} & = u \Delta x \\
\end{align*}

\begin{align*}
\tilde{\rho} & = \int _{-\infty} ^{\infty} \rho e ^{-ikx} dx \\
\tilde{\rho} _x & = \int _{-\infty} ^{\infty} \left( \frac{\partial}{\partial x} \rho \right) e ^{-ikx} dx \\
\tilde{\rho} _{xx} & = \int _{-\infty} ^{\infty} \left( \frac{\partial ^2}{\partial x ^2} \rho \right) e ^{-ikx} dx \\
\end{align*}

Proof of the differentials Fourier transformed; 

\begin{align*}
\tilde{\rho} _x & = \int _{-\infty} ^{\infty} \left( \frac{\partial}{\partial x} \rho \right) e ^{-ikx} dx \\
& = \left[ \rho e ^{-ikx} \right] _{- \infty } ^{\infty} + ik \tilde{\rho} \\
\\
\tilde{\rho} _{xx} & = \int _{-\infty} ^{\infty} \left( \frac{\partial ^2}{\partial x ^2} \rho \right) e ^{-ikx} dx \\
& = \left[ \rho _x e^{-ikx} \right] _{-\infty} ^{\infty} + ik \int e ^{-ikx} \rho _x dx \\
& = \left[ \rho _x e^{-ikx} \right] _{-\infty} ^{\infty} + ik \left( 
\left[ \rho e ^{-ikx} \right] _{- \infty } ^{\infty} + ik \tilde{\rho} \right) \\
& = \left[ \rho _x e^{-ikx} \right] _{-\infty} ^{\infty} + ik \left[ \rho e ^{-ikx} \right] _{- \infty } ^{\infty} - k^2 \tilde{\rho}
\end{align*}

\begin{align*}
\dot{\tilde{\rho}} & = - \frac{\tilde{u} \Delta x k^2}{2} \tilde{\rho} - ik \tilde{u} \tilde{\rho} \\
\tilde{\rho} & = A \exp \left( - \tilde{u} k \left( \frac{k \Delta x}{2} + i \right) t \right) \\
\tilde{\rho} (k, 0) & = A \\
\tilde{\rho} (k, 0) & = \int _{- \infty} ^{\infty} \rho (x, 0) e^{-ikx} dx \\
& = \int _{- \infty} ^{\infty} \delta (x - x_0)  e^{-ikx} dx \\
& = e^{-ik x_0} 
\end{align*}

\begin{equation}
\tilde{\rho}  = e^{-ik x_0} \exp \left( - \tilde{u} k \left( \frac{k \Delta x}{2} + i \right) t \right) \\
\end{equation}

Need to do the inverse Fourier transform to get back to concentration space.
 

\begin{align*}
\rho & = \int _{- \infty } ^{\infty} \exp \left( - \tilde{u} k \left( \frac{k \Delta x}{2} + i \right) t -ikx_0 \right) e^{ikx} dk \\
& = \sqrt{\frac{2 \pi}{\Delta x \tilde{u} t}} \exp \left( - \frac{(\tilde{u} t - x + x_0 )^2}{2 \Delta x \tilde{u} t} \right)
\end{align*}

This is the solution, which gives a Gaussian shape propagating. 

\subsection{Sanity check with differentiation}

\begin{align*}
\rho & = \sqrt{\frac{2 \pi}{\Delta x \tilde{u} t}} \exp \left( - \frac{(\tilde{u} t - x + x_0 )^2}{2 \Delta x \tilde{u} t} \right) \\
& = \frac{C}{\sqrt{t}} \exp \left( - \frac{(\tilde{u} t - x + x_0 )^2}{Bt} \right) \\
& = \frac{C}{\sqrt{t}} \exp \left( - \frac{(\tilde{u} t)^2 + (x_0 - x)^2 + 2 \tilde{u}t (x_0 - x)}{Bt} \right) \\
& = \frac{C}{\sqrt{t}} \exp \left( - \left[ \frac{\tilde{u} ^2 t}{B} + \frac{(x_0 - x)^2}{Bt} + \frac{2 \tilde{u} (x_0 - x)}{B} \right] \right) \\
& = \frac{C}{\sqrt{t}} e^{- \alpha} e^{- \beta} e^{- \gamma} \\
\end{align*}

\begin{align*}
\partial _t \rho & = \rho \left( - \frac{1}{2t} - \frac{\tilde{u} ^2}{B} + \frac{(x_0 - x)^2}{Bt^2} \right) \\
\partial _x \rho & = \rho \left( \frac{2(x_0 -x )}{Bt} + \frac{2 \tilde{u}}{Bt} \right) \\
\partial_{xx} \rho & = \rho \left( \left[ \frac{2(x_0 -x )}{Bt} + \frac{2 \tilde{u}}{Bt} \right] ^2 - \frac{2}{Bt} \right)
\end{align*}

\begin{align*}
\dot{\rho} & = \frac{\tilde{u} \Delta x}{2} \partial _{xx} \rho - \tilde{u} \partial _x \rho \\
\end{align*}

\begin{align*}
\left( - \frac{1}{2t} - \frac{\tilde{u} ^2}{B} + \frac{(x_0 - x)^2}{Bt^2} \right) & = \frac{\tilde{u} \Delta x}{2} \left( \frac{2(x_0 -x )}{Bt} + \frac{2 \tilde{u}}{Bt} \right) - \tilde{u} \left( \left[ \frac{2(x_0 -x )}{Bt} + \frac{2 \tilde{u}}{Bt} \right] ^2 - \frac{2}{Bt} \right) \\
\left( - \frac{1}{2t} - \frac{\tilde{u} ^2}{B} + \frac{(\tilde{x})^2}{Bt^2} \right) & = \frac{B}{4} \left( \frac{2(\tilde{x})}{Bt} + \frac{2 \tilde{u}}{Bt} \right) - \tilde{u} \left( \left[ \frac{2(\tilde{x} )}{Bt} + \frac{2 \tilde{u}}{Bt} \right] ^2 - \frac{2}{Bt} \right) \\
\left( - \frac{1}{2t} - \frac{\tilde{u} ^2}{B} + \frac{(\tilde{x})^2}{Bt^2} \right) & = \frac{1}{2t} (\tilde{x} + \tilde{u} ) - \tilde{u} \left( \frac{4}{B^2 t^2}( \tilde{x} ^2 + \tilde{u}^2 + 2 \tilde{u} \tilde{x} ) - \frac{2}{Bt} \right)
\end{align*}

It doesn't work! something has gone wrong somewhere. 

Turns out it did work, something went wrong in the algebra. 

\subsection*{Constraints on the Solution}

From the differentiation not working, can imply that this imposes some constraints on the constants. 

The concentration must also also be conserved; 

\begin{equation}
\int _0 ^\infty \rho (x,t ) dx = 1 \quad \forall t
\end{equation}

\begin{align*}
\dot{\rho} & = \frac{\tilde{u} \Delta x}{2} \frac{\partial ^2}{\partial x ^2} \rho - \tilde{u} \frac{\partial}{\partial x} \rho \\
\end{align*}

From the Fourier analysis we assume a solution; 

\begin{equation}
\rho = \frac{C}{\sqrt{t}} \exp \left( - \frac{(At - (x-x_0)^2}{Bt} \right)
\end{equation}

Doing the integral thing 

\begin{align*}
\frac{1}{2} C \sqrt{\pi B} \left( \text{Erf} \left( \frac{x_0 + At}{\sqrt{B} \sqrt{t}} \right) + 1 \right) & = 1 \\ 
x_0 & = 0 \\
C \sqrt{\pi B} \left( \text{Erf} \left( \frac{A \sqrt{t}}{\sqrt{B}} \right) + 1 \right) & = 2
\end{align*}

The error function tends to 1 quickly, so even after a small amount of time, its reasonable to replace it with 1. 

\begin{equation}
C \sqrt{B} = \frac{1}{\sqrt{\pi}}
\end{equation}

This gives us our first constraint. 

\subsection{Numerically Solving the PDE}

\begin{align*}
\dot{\rho} & = \frac{\tilde{u} \Delta x}{2} \frac{\partial ^2 \rho}{\partial x^2} - \tilde{u} \frac{\partial \rho}{\partial x} \\
\tilde{u} & = u \Delta	x \\
\end{align*}

Need to discretise the system. 

\begin{align*}
x_i & =  ih \\
t_j & = jk \\
\dot{\rho} & = \frac{ \rho _{i j+1} - \rho_{ij} }{k} \\
\frac{\partial \rho}{\partial x} & = \frac{\rho _{i+1 j} - \rho _{ij}}{h} \\
\frac{\partial ^2 \rho}{\partial x ^2} & = \frac{\rho _{i+1 j} - 2 \rho _{ij} + \rho_{i-1 j}}{h^2} \\
\end{align*}

\begin{align*}
\frac{ \rho _{i j+1} - \rho_{ij} }{k} & = \frac{\tilde{u} \Delta x}{2} \left( \frac{\rho _{i+1 j} - 2 \rho _{ij} + \rho_{i-1 j}}{h^2} \right) - \tilde{u} \left( \frac{\rho _{i+1 j} - \rho _{ij}}{h} \right)
\rho _{i j+1} \\
\rho_{ij+1}& =  \rho _{ij} + \frac{k \tilde{u} \Delta x}{2 h^2} \rho _{i +1 j} - \frac{k \tilde{u} \Delta x}{2 h^2} \rho _{ij} + \frac{k \tilde{u \Delta x}}{2 h^2} \rho _{i-1 j} - \frac{\tilde{u} k}{h} \rho _{i+1 j} + \frac{\tilde{u} k}{h} \rho_{ij} \\
& = \left( 1 + \frac{\tilde{u} k }{h} - \frac{k \tilde{u} \Delta x}{2 h^2} \right) \rho _{ij} + \left( \frac{k \tilde{u} \Delta x}{2 h^2} - \frac{\tilde{u} k}{h} \right) \rho _{i+1 j} + \frac{k \tilde{u} \Delta x}{2 h^2} \rho _{i-1 j} \\
& = \left( 1 + \alpha - \beta \right) \rho _{ij} + \left( \beta - \alpha \right) \rho _{i+1 j} + \beta \rho _{i-1 j} \\
\end{align*}

\end{document}